tests/DoubleCountBy/ListProofs.v
@@ -1,0 +1,99 @@
+(****************************************************************************)
+(* Copyright 2021 The Project Oak Authors                                   *)
+(*                                                                          *)
+(* Licensed under the Apache License, Version 2.0 (the "License")           *)
+(* you may not use this file except in compliance with the License.         *)
+(* You may obtain a copy of the License at                                  *)
+(*                                                                          *)
+(*     http://www.apache.org/licenses/LICENSE-2.0                           *)
+(*                                                                          *)
+(* Unless required by applicable law or agreed to in writing, software      *)
+(* distributed under the License is distributed on an "AS IS" BASIS,        *)
+(* WITHOUT WARRANTIES OR CONDITIONS OF ANY KIND, either express or implied. *)
+(* See the License for the specific language governing permissions and      *)
+(* limitations under the License.                                           *)
+(****************************************************************************)
+
+Require Import Coq.Strings.String.
+Require Import Coq.NArith.NArith.
+Require Import Coq.Lists.List.
+Require Import Coq.Vectors.Vector.
+Import ListNotations VectorNotations.
+Local Open Scope list_scope.
+
+Require Import ExtLib.Structures.Monads.
+Export MonadNotation.
+
+Require Import Cava.Cava.
+Require Import Cava.ListUtils.
+Require Import Cava.Tactics.
+Require Import Cava.Acorn.CavaClass.
+Require Import Cava.Acorn.Circuit.
+Require Import Cava.Acorn.Identity.
+Require Import Cava.Acorn.Combinational.
+Require Import Cava.Acorn.Combinators.
+Require Import Cava.Lib.UnsignedAdders.
+
+Require Import DoubleCountBy.DoubleCountBy.
+
+Existing Instance CombinationalSemantics.
+
+Definition bvadd {n} (a b : Vector.t bool n) : Vector.t bool n :=
+  N2Bv_sized n (Bv2N a + Bv2N b).
+
+Definition bvsum {n} (l : list (Vector.t bool n)) : Vector.t bool n :=
+  fold_left bvadd l (N2Bv_sized n 0).
+
+Definition bvaddc {n} (a b : Vector.t bool n) : Vector.t bool n * bool :=
+  let sum := (Bv2N a + Bv2N b)%N in
+  let carry := (Bv2N a <? sum mod (2 ^ N.of_nat n))%N in
+  (N2Bv_sized n sum, carry).
+
+Definition bvsumc {n} (l : list (Vector.t bool n)) : Vector.t bool n * bool :=
+  fold_left (fun '(acc,_) => bvaddc acc) l (N2Bv_sized n 0, false).
+
+Definition count_by_spec (i : list (Vector.t bool 8)) : list (Vector.t bool 8 * bool) :=
+  map (fun t => bvsumc (firstn t i)) (seq 1 (length i)).
+
+Definition double_count_by_spec (i : list (Vector.t bool 8)) : list (Vector.t bool 8 * bool) :=
+  map (fun t => bvsumc (firstn t i)) (seq 1 (length i)).
+
+Lemma addN_correct {n} (x y : combType (Vec Bit n)) :
+  unIdent (addN (x, y)) = N2Bv_sized n (Bv2N x + Bv2N y).
+Admitted.
+Hint Rewrite @addN_correct : simpl_ident.
+
+Lemma ltV_correct {n m} x y :
+  unIdent (ltV (n:=n) (m:=m) (x, y)) = (Bv2N x <? Bv2N y)%N.
+Admitted.
+Hint Rewrite @ltV_correct : simpl_ident.
+
+Lemma addC_correct {n} (x y : combType (Vec Bit n)) :
+  unIdent (addC (x, y)) = (N2Bv_sized n (Bv2N x + Bv2N y),
+                           (Bv2N x <? (Bv2N x + Bv2N y) mod (2 ^ N.of_nat n)))%N.
+Proof.
+  cbv [addC]. cbv [CombinationalSemantics].
+  simpl_ident. rewrite Bv2N_N2Bv_sized_modulo.
+  reflexivity.
+Qed.
+
+Lemma incrN_correct {n} (x : combType (Vec Bit (S n))) :
+  unIdent (incrN x) = N2Bv_sized (S n) (Bv2N x + 1).
+Proof.
+  cbv [incrN].
+  cbv [CombinationalSemantics peel unpeel unsignedAdd unsignedAddBool constant].
+  simpl_ident. cbn [Nat.max Nat.add Bv2N N.succ_double].
+  (* just proof about shiftout from here *)
+Admitted.
+
+Print count_by.
+Lemma count_by_correct (input : list (combType (Vec Bit 8))) :
+  multistep count_by (tt, (defaultCombValue _, defaultCombValue _)) input
+  = count_by_spec input.
+
+
+
+Print multistep.
+Check addN.
+Check (multistep (Comb addN)).
+
